#+TITLE: Surface Metric
#+OPTIONS: toc:nil num:nil

* Riemannian Metric
** Riemannian Metric

The Riemannian metric of a surface completely determines the geometry of the surface.

** Metric (First Fundamental Form)

#+BEGIN_env defn
The (Riemmanian) metric \(g\) on \(S\) is the inner product \(g_p\) at each point \(p \in S\) defined for tangent vectors \(V, W \in T_p S \subseteq \RR^3\) by
\[
g_p(V, W) = \ip{V}{V}_{\RR^3}.
\]
#+END_env

** Coordinate Expression of Metric

\[
V = c^1 \partial_{x_1} \varphi + c^2 \partial_{x_2} \varphi, \quad W = d^1 \partial_{x_1} \varphi + d^2 \partial_{x_2} \varphi
\]

\begin{equation*}
\begin{split}
g(V, W) &= \ip{c_1 \frac{\partial \varphi}{\partial x_1} + c_2 \frac{\partial \varphi}{\partial x_2}}{d_1 \frac{\partial \varphi}{\partial x_1} + d_2 \frac{\partial \varphi}{\partial x_2}} \\
&= c_1 d_1 \ip{\frac{\partial \varphi}{\partial x_1}}{\frac{\partial \varphi}{\partial x_1}} + c_2 d_2 \ip{\frac{\partial \varphi}{\partial x_2}}{\frac{\partial \varphi}{\partial x_2}} \\
&\quad + (c_1d_2 + c_2 d_1) \ip{\frac{\partial \varphi}{\partial x_1}}{\frac{\partial \varphi}{\partial x_2}} \\
&= c_1 d_1 g_{11} + c_2 d_2 g_{22} + (c_1 d_2 + c_2 d_1) g_{12}.
\end{split}
\end{equation*}

** Matrix Form in Local Coordinates

\[
g(U, V) = U^T g V
\]

\begin{equation*}
g = \begin{pmatrix}
g_{11} & g_{12} \\
g_{21} & g_{22}
\end{pmatrix}
=
\begin{pmatrix}
\ip{\frac{\partial \varphi}{\partial x_1}}{\frac{\partial \varphi}{\partial x_1}} &  \ip{\frac{\partial \varphi}{\partial x_1}}{\frac{\partial \varphi}{\partial x_2}} \\
\ip{\frac{\partial \varphi}{\partial x_2}}{\frac{\partial \varphi}{\partial x_1}} & \ip{\frac{\partial \varphi}{\partial x_2}}{\frac{\partial \varphi}{\partial x_2}}
\end{pmatrix}
\end{equation*}

\((g_{ij})\) is /positive definite/ and /symmetric/.

** Change of Coordinates

Change of coords \(\tau = \varphi^{-1} \circ \psi: \RR^2 \to \RR^2\):
\begin{equation*}
\begin{split}
g^{\psi}_{ab} &= g^{\varphi \circ \tau}_{ab} \\
&= \ip{\partial_{y^a} (\varphi \circ \tau)}{\partial_{y^b} (\varphi \circ \tau)} \\
&= \ip{\sum_i \partial_{x^i} \varphi \partial_{y^a} \tau^i}{\sum_j \partial_{x^j} \varphi \partial_{y^b} \tau^j} \\
&= \sum_{ij} g_{ij} \partial_{y^a} \tau^i \partial_{y^b} \tau^j
\end{split}
\end{equation*}

** Matrix Change of Coordinates

\begin{equation*}
\begin{split}
g^{\varphi \circ \tau}(X, Y) &= \ip{d(\varphi \circ \tau) \cdot X}{d(\varphi \circ \tau) \cdot Y} \\
&= \ip{d\varphi(d\tau \cdot X)}{d\varphi(d\tau \cdot y)} \\
&= g^{\varphi} (d\tau \cdot X, d\tau \cdot Y).
\end{split}
\end{equation*}

\[
g^{\varphi \circ \tau} = d\tau^T g d\tau
\]

* Examples
** Examples
** Euclidean Metric

#+BEGIN_env eg
\[
\varphi(u, v) = (u, v, 0)
\]

Then \(g = \delta\)

i.e. \(g_{ij} = \delta_{ij}\)
#+END_env

** Sphere Metric: Spherical

#+BEGIN_env eg
\begin{align*}
\varphi (\theta, \phi) &= (\sin\phi \cos\theta, \sin\phi \sin\theta, \cos\phi) \\
e_{\theta} &= (-\sin\phi\sin\theta, \sin\phi\cos\theta, 0) \\
e_{\phi} &= (\cos\phi \cos\theta, \cos\phi \sin\theta, -\sin\phi)
\end{align*}

\begin{equation*}
g = \begin{pmatrix}
\sin^2 \phi & 0 \\
0 & 1
\end{pmatrix}
\end{equation*}
#+END_env

** Sphere Metric: Cylindrical

#+BEGIN_env eg
\begin{align*}
\varphi (\eta, r) &= (\sqrt{1-r^2} \cos\eta, \sqrt{1-r^2} \sin\eta, r) \\
e_{\eta} &= (-\sqrt{1-r^2} \sin \eta, \sqrt{1-r^2} \cos \eta, 0) \\
e_r &= \left(\tfrac{-r}{\sqrt{1-r^2}} \cos \eta, \tfrac{-r}{\sqrt{1-r^2}} \sin \eta, 1 \right)
\end{align*}

\begin{equation*}
g = \begin{pmatrix}
1 - r^2 & 0 \\
0 & \tfrac{1}{1-r^2}
\end{pmatrix}
\end{equation*}
#+END_env

** Cylindrical to Spherical

\[
(\eta, r) = (\theta, \cos \phi)
\]

\begin{equation*}
\begin{split}
g^{\operatorname{Cyl}} &= d\tau^T g^{\SS^2} d\tau \\
&= \begin{pmatrix}
1 & 0 \\
0 & \tfrac{-1}{\sqrt{1-r^2}}
\end{pmatrix}
\begin{pmatrix}
\sin^2 \phi & 0 \\
0 & 1
\end{pmatrix}
\begin{pmatrix}
1 & 0 \\
0 & \tfrac{-1}{\sqrt{1-r^2}}
\end{pmatrix} \\
&= \begin{pmatrix}
\sin^2 \phi & 0 \\
0 & \tfrac{1}{1 - r^2}
\end{pmatrix}
= \begin{pmatrix}
1-r^2 & 0 \\
0 & \tfrac{1}{1 - r^2}
\end{pmatrix}
\end{split}
\end{equation*}

** Paraboloid

#+BEGIN_env eg
\begin{align*}
\varphi(u, v) &= (u, v, u^2 + v^2) \\
e_u &= (1, 0, 2u) \\
e_v &= (0, 1, 2v)
\end{align*}

\begin{equation*}
g = \begin{pmatrix}
1 + 4u^2 & 4uv \\
4uv & 1 + 4v^2
\end{pmatrix}
\end{equation*}
#+END_env

