#+OPTIONS: toc:nil num:nil
#+BEGIN_export html
---
title: Surface Geometry
short_title: Surface Geometry
---
#+END_export

#+LaTeX_class: article_no_macros
#+LaTeX_Header: \usepackage{pabnotes}
#+LaTeX_Header: \newcommand{\weeknum}{05}
#+LaTeX_Header: \newcommand{\topic}{Surface Geometry}

#+BEGIN_export html
<ul>
<li><a href="{{ '/slides/surface_metric' | relative_url }}" target="_blank">Surfaces Metric Slides</a></li>

<li><a href="{{ '/slides/surface_geometry' | relative_url }}" target="_blank">Surfaces Geometry Slides</a></li>
<!-- <li><a href="{{ '/pdf/surface_geometry.pdf' | relative_url }}" target="_blank">Surfaces Geometry PDF Notes</a></li>-->
</ul>
#+END_export

* Riemannian Metric                                                :noexport:

The Riemannian metric of a surface completely determines the geometry of a regular surface.

#+BEGIN_env defn
The (Riemmanian) metric \(g\) on \(S\) is the inner product \(g_p\) at each point \(p \in S\) defined for tangent vectors \(V, W \in T_p S \subseteq \RR^3\) by
\[
g_p(V, W) = \ip{V}{V}_{\RR^3}.
\]
#+END_env

With respect to local coordinates (i.e. in a local parametrisation) we may write

\[
V = c^1 \partial_{x_1} \varphi + c^2 \partial_{x_2} \varphi, \quad W = d^1 \partial_{x_1} \varphi + d^2 \partial_{x_2} \varphi
\]

\begin{equation*}
\begin{split}
g(V, W) &= \ip{c_1 \frac{\partial \varphi}{\partial x_1} + c_2 \frac{\partial \varphi}{\partial x_2}}{d_1 \frac{\partial \varphi}{\partial x_1} + d_2 \frac{\partial \varphi}{\partial x_2}} \\
&= c_1 d_1 \ip{\frac{\partial \varphi}{\partial x_1}}{\frac{\partial \varphi}{\partial x_1}} + c_2 d_2 \ip{\frac{\partial \varphi}{\partial x_2}}{\frac{\partial \varphi}{\partial x_2}} \\
&\quad + (c_1d_2 + c_2 d_1) \ip{\frac{\partial \varphi}{\partial x_1}}{\frac{\partial \varphi}{\partial x_2}} \\
&= c_1 d_1 g_{11} + c_2 d_2 g_{22} + (c_1 d_2 + c_2 d_1) g_{12}.
\end{split}
\end{equation*}

Note that this latter expression may be written
\[
g(U, V) = U^T g^{\varphi} V
\]
where \(g^{\varphi}\) is the matrix
\begin{equation*}
g^{\varphi} = \begin{pmatrix}
g_{11} & g_{12} \\
g_{21} & g_{22}
\end{pmatrix}
=
\begin{pmatrix}
\ip{\frac{\partial \varphi}{\partial x_1}}{\frac{\partial \varphi}{\partial x_1}} &  \ip{\frac{\partial \varphi}{\partial x_1}}{\frac{\partial \varphi}{\partial x_2}} \\
\ip{\frac{\partial \varphi}{\partial x_2}}{\frac{\partial \varphi}{\partial x_1}} & \ip{\frac{\partial \varphi}{\partial x_2}}{\frac{\partial \varphi}{\partial x_2}}
\end{pmatrix}
\end{equation*}

The matrix \((g^{\varphi}_{ij})\) is /positive definite/ and /symmetric/.


Whenever we obtain expressions in coordinates, we should check to see what happens when we change coordinates. Letting \(\tau = \varphi^{-1} \circ \psi: \RR^2 \to \RR^2\) denote the change of parameters. Then
\begin{equation*}
\begin{split}
g^{\psi}_{ab} &= g^{\varphi \circ \tau}_{ab} \\
&= \ip{\partial_{y^a} (\varphi \circ \tau)}{\partial_{y^b} (\varphi \circ \tau)} \\
&= \ip{\sum_i \partial_{x^i} \varphi \partial_{y^a} \tau^i}{\sum_j \partial_{x^j} \varphi \partial_{y^b} \tau^j} \\
&= \sum_{ij} g_{ij} \partial_{y^a} \tau^i \partial_{y^b} \tau^j
\end{split}
\end{equation*}
Somewhat more compactly, we may write this as
\begin{equation*}
\begin{split}
g^{\varphi \circ \tau}(X, Y) &= \ip{d(\varphi \circ \tau) \cdot X}{d(\varphi \circ \tau) \cdot Y} \\
&= \ip{d\varphi(d\tau \cdot X)}{d\varphi(d\tau \cdot y)} \\
&= g^{\varphi} (d\tau \cdot X, d\tau \cdot Y).
\end{split}
\end{equation*}
That is,
\[
g^{\varphi \circ \tau} = d\tau^T g^{\varphi} d\tau
\]

* Examples                                                         :noexport:

Let's examine some examples to see what it's all about.

#+BEGIN_env eg :title "Euclidean Metric"
\[
\varphi(u, v) = (u, v, 0)
\]

Then \(g = \delta\). That is \(g_{ij} = \delta_{ij}\) is the dirac-delta that is \(1\) when \(i=j\) and \(0\) when \(i \neq j\). In other words, the identity matrix.
#+END_env

#+BEGIN_env eg :title "Sphere Metri - Spherical Coordinates"
\begin{align*}
\varphi (\theta, \phi) &= (\sin\phi \cos\theta, \sin\phi \sin\theta, \cos\phi) \\
e_{\theta} &= (-\sin\phi\sin\theta, \sin\phi\cos\theta, 0) \\
e_{\phi} &= (\cos\phi \cos\theta, \cos\phi \sin\theta, -\sin\phi)
\end{align*}

\begin{equation*}
g = \begin{pmatrix}
\sin^2 \phi & 0 \\
0 & 1
\end{pmatrix}
\end{equation*}
#+END_env

#+BEGIN_env eg :title "Sphere Metric - Cylindrical Coordinates"
\begin{align*}
\varphi (\eta, r) &= (\sqrt{1-r^2} \cos\eta, \sqrt{1-r^2} \sin\eta, r) \\
e_{\eta} &= (-\sqrt{1-r^2} \sin \eta, \sqrt{1-r^2} \cos \eta, 0) \\
e_r &= \left(\tfrac{-r}{\sqrt{1-r^2}} \cos \eta, \tfrac{-r}{\sqrt{1-r^2}} \sin \eta, 1 \right)
\end{align*}

\begin{equation*}
g = \begin{pmatrix}
1 - r^2 & 0 \\
0 & \tfrac{1}{1-r^2}
\end{pmatrix}
\end{equation*}
#+END_env

To change basis between coordinates, note that we have

\[
(\eta, r) = (\theta, \cos \phi).
\]

From a previous section we obtained the transition map which gives
\begin{equation*}
\begin{split}
g^{\operatorname{Cyl}} &= d\tau^T g^{\SS^2} d\tau \\
&= \begin{pmatrix}
1 & 0 \\
0 & \tfrac{-1}{\sqrt{1-r^2}}
\end{pmatrix}
\begin{pmatrix}
\sin^2 \phi & 0 \\
0 & 1
\end{pmatrix}
\begin{pmatrix}
1 & 0 \\
0 & \tfrac{-1}{\sqrt{1-r^2}}
\end{pmatrix} \\
&= \begin{pmatrix}
\sin^2 \phi & 0 \\
0 & \tfrac{1}{1 - r^2}
\end{pmatrix} \\
&= \begin{pmatrix}
1-r^2 & 0 \\
0 & \tfrac{1}{1 - r^2}
\end{pmatrix}
\end{split}
\end{equation*}
where in the last line we used that the \(z\)-coordinate is \(r = r = \cos\phi\) in the two different parametrisations, hence \(\sin^2 \phi = 1 - \cos^2\phi = 1 - r^2\).

#+BEGIN_env eg
\begin{align*}
\varphi(u, v) &= (u, v, u^2 + v^2) \\
e_u &= (1, 0, 2u) \\
e_v &= (0, 1, 2v)
\end{align*}

\begin{equation*}
g = \begin{pmatrix}
1 + 4u^2 & 4uv \\
4uv & 1 + 4v^2
\end{pmatrix}
\end{equation*}
#+END_env

* Angle and Length                                                 :noexport:
** Angle and Length

We can define angle and length by using the metric \(g\).

#+BEGIN_env defn
Let \(X\) be a tangent vector. Then it's length is defined to be
\[
\abs{X}_g := \sqrt{g(X, X)}.
\]
#+END_env

Before defining the angle, let us recall the Cauchy-Schwarz inequality for inner-products \(g\):
#+BEGIN_lemma
\[
\abs{g(X, Y)} \leq \abs{X}\abs{Y}.
\]
#+END_lemma

Notice that for \(X, Y \ne 0\)
\[
\frac{g(X, Y)}{\abs{X}\abs{Y}} \in [-1, 1].
\]
Now we may define the angle.

#+BEGIN_env defn
The angle, \(\theta\) between two tangent vectors \(X, Y\) (at the same point \(x \in S\)!) is defined by
\[
\cos \theta = \frac{g(X, Y)}{\abs{X}\abs{Y}} = g\left(\frac{X}{\abs{X}}, \frac{Y}{\abs{Y}}\right)
\]
where to obtain \(\theta\) we choose a local inverse for \(\cos\) such as \(\arccos\) giving an angle in \([0, \pi]\).
#+END_env

** Arc Length

#+BEGIN_defn
Let \(\gamma : (a, b) \to S\) be a smooth curve. The /arc-length/ of \(\gamma\) is
\[
L(\gamma) = \int_a^b \abs{\gamma'(t)} dt = \int_a^b \sqrt{g_{\gamma(t)} (\gamma'(t), \gamma'(t))} dt.
\]
#+END_defn

This is just the arc-length in \(\RR^3\) but expressed in terms of \(g\).

** Example: Paraboloid

#+BEGIN_env eg
Let \(\gamma(t) = (t, 0, t^2)\), \(\mu (t) = \varphi^{-1} \circ \gamma (t) = (t, 0)\)

\begin{equation*}
\begin{split}
\abs{\gamma'}_{\RR^3}^2 &= \abs{\mu'}_{g(\mu(t))}^2 =
\begin{pmatrix}
1 & 0
\end{pmatrix}
\begin{pmatrix}
1 + 4u^2 & 4uv \\
4uv & 1 + 4v^2
\end{pmatrix}
\begin{pmatrix}
1 \\ 0
\end{pmatrix} \\
&= \begin{pmatrix}
1 & 0
\end{pmatrix}
\begin{pmatrix}
1 + 4t^2 & 0 \\
0 & 1
\end{pmatrix}
\begin{pmatrix}
1 \\ 0
\end{pmatrix} \\
&= 1 + 4t^2
\end{split}
\end{equation*}

\[
L(\gamma) = \int \sqrt{1 + 4t^2} dt
\]
#+END_env

** Example: Paraboloid

#+BEGIN_env eg
At \(p = (u, v, u^2 + v^2)\)

\begin{align*}
g(\gamma_u', \gamma_u') &= 1 + 4u^2 \\
g(\gamma_v', \gamma_v') &= 1 + 4v^2 \\
g(\gamma_u', \gamma_v') &= 4uv
\end{align*}

\[
\cos \theta(\gamma_u', \gamma_v') = \frac{4uv}{\sqrt{1+4u^2}\sqrt{1+4v^2}}
\]

#+END_env
* Area                                                             :noexport:
** Area

Area is also determined by the metric.

** Area

Let
\[
X_u = d\varphi (e_u) = \partial_u \varphi, \quad X_v = d\varphi (e_v) = \partial_v \varphi
\]
be coordinate vectors.

Since \(d\varphi\) is injective, \(X_u, X_v\) form a basis for \(T_x M\).

** Area

Parallelogram: \(X_u \wedge X_v \subseteq T_x M\)

Taking a small rectangle \(R = \{(u, v) \in (u_0, u_0 + \Delta u) \times (v_0, v_0 + \Delta v)\}\), we approximate the area of \(\varphi(R) \subseteq S\) by
\begin{equation*}
\begin{split}
\text{Area} (S) &\simeq \text{Area} (X_u \wedge X_v) \\

&= \abs{X_u \times X_v} \text{Area}(R) \\
&= \abs{X_u \times X_v} \Delta u \Delta v.
\end{split}
\end{equation*}

** Area

Note that \(\abs{X_u \times X_v}^2 = \det \lambda^T \lambda = \det g\) where \(\lambda = (X_u \quad X_v)\)!

Area is the limit of a Riemann sum: for any region \(\Omega = \varphi(W)\)
\[
\text{Area} (\Omega) = \int_W \sqrt{\det g(u, v)} du dv.
\]

** Cylinder to Sphere
* Orientation And The Gauss Map                                    :noexport:
** Orientation And The Gauss Map
** Orientation of Euclidean Space

#+BEGIN_env defn
An orientation on \(\RR^n\) is an equivalence class of /ordered/ bases \(\mathcal{E} = (e_1, \cdots, e_n)\) where \(\mathcal{E} \sim \mathcal{F}\) if the change of basis matrix \(A_{\mathcal{E}\mathcal{F}}\) has positive determinant.
#+END_env

\pause

Since \(\det \left(A_{\mathcal{E}\mathcal{F}} A_{\mathcal{F}\mathcal{G}}\right) = \det \left(A_{\mathcal{E}\mathcal{F}}\right) \det\left(A_{\mathcal{F}\mathcal{G}}\right)\), we do indeed have an equivalence relation, and there are /precisely two equivalence classes/.

\pause

\begin{example}
Compute the change of basis from \(\mathcal{E} = (e_1, e_2)\) to \((e_1, e_1 + e_2), \quad (e_1, -e_2), \quad (e_2, e_1).\)
\end{example}

\pause

\begin{example}
Right hand orientation: \((e_1, e_2, e_3), (e_1, e_3, -e_2), \dots\)

Left hand orientation: \((e_2, e_1, e_3), (e_1, -e_2, e_3), \dots\)
\end{example}

** Orientation preserving and reversing linear maps

Choose an orientation \(\mathcal{O} = \{e_1, \cdots, e_n\}\) on \(\RR^n\).

#+BEGIN_env defn
An /invertible/ linear map \(T : \RR^n \to \RR^n\) is orientation preserving if \(T(\mathcal{O}) = \mathcal{O}\). That is, if
\[
\det \begin{pmatrix}
T(e_1), \cdots, T(e_n)
\end{pmatrix}
= \det \begin{pmatrix}
e_1, \cdots, e_n
\end{pmatrix}
\]
or equivalently if \(\det T > 0\).
#+END_env

\pause

\begin{example}
\[
\text{Preserving:} \quad
T = \begin{pmatrix}
1 & 0 \\
0 & 1
\end{pmatrix}, \quad
T = \begin{pmatrix}
1 & 1 \\
1 & 0
\end{pmatrix}, \quad
T = \begin{pmatrix}
2 & 1 \\
3 & 5
\end{pmatrix}.
\]
\[
\text{Reversing:} \quad
T = \begin{pmatrix}
1 & 0 \\
0 & -1
\end{pmatrix}, \quad
T = \begin{pmatrix}
0 & 1 \\
1 & 0
\end{pmatrix}, \quad
T = \begin{pmatrix}
2 & 1 \\
3 & 1
\end{pmatrix}.
\]
\end{example}

** Orientation of the tangent plane
*** Tangent Plane Orientations
**** Text
      :PROPERTIES:
      :BEAMER_col: 0.5
      :END:

Local parametrisation: \(\varphi : U \to S\).
\[
\left(\frac{\partial \varphi}{\partial u}, \frac{\partial \varphi}{\partial v}\right), \quad \left(\frac{\partial \varphi}{\partial v}, \frac{\partial \varphi}{\partial u}\right)
\]
**** Picture
      :PROPERTIES:
      :BEAMER_col: 0.5
      :END:

#+BEGIN_center
#+ATTR_LATEX: :width .9\textwidth :height .4\textheight
[[file:img/oriented_tangent_plane.png]]
#+END_center

\pause
*** Definition
The orientation induced by \(\varphi\) is /compatible/ with the orientation induced by \(\psi\) if \(\det d(\psi \circ \phi^{-1}) > 0\).
\pause
A regular surface, \(S\) is /orientable/ if there is a cover \(\varphi_{\alpha} : U_{\alpha} \to S\) such that \(\det(\tau_{\alpha\beta}) > 0\) for all \(\alpha, \beta\).

** Examples

- The sphere is orientable
- The \mobius{} strip is /not/ orientable
- Graphs, are orientable
- Inverse images of regular point are orientable: here \(F: \RR^3 \to \RR\), \(S = F^{-1}(0)\) where \(dF_x\) has maximal rank (i.e. rank \(1\)) for all \(p \in \RR^3\) such that \(F(p) = 0\).

** Orientation of surfaces

#+BEGIN_theorem
A surface \(S\) is orientable if and only if there is a differentiable field, \(N\) of unit normal vectors. That is, if and only there exists a differentiable map \(N : S \to \RR^3\) such that \(\abs{N(x)} = 1\) for all \(x \in S\) and such that \(N(x) \perp X\) for all $X \in T_x S$.
#+END_theorem

\pause

*Remember there are precisely two orientations!*

\pause

There are two possible unit normal fields, \(N\) and \(-N\). Choosing an orientation is equivalent to choosing a normal field.

\pause

- The proof of the theorem follows from the following lemma:

#+BEGIN_lemma
Let \(\varphi (u, v) : U \subseteq \RR^2 \to S\) and \(\psi (s, t) : V \subseteq \RR^2 \to S\) be local parametrisations. Then
\[
\partial_u \varphi \times \partial_v \varphi = \left[\det d(\psi^{-1} \circ \varphi)\right] \partial_s \psi \times \partial_t \psi.
\]
#+END_lemma

** Gauss Map

#+BEGIN_env defn
 An orientable surface \(S\) along with a choice of orientation is called an /oriented surface/.
#+END_env

\pause

#+BEGIN_env defn
Let \(S\) be an oriented surface. The /Gauss Map/ is the unit normal map
\[
x \in S \mapsto N(x) \in \sphere^2 = \{X \in \RR^3 : \|X\| = 1\}.
\]
#+END_env

\pause

With respect to a local parametrisation
\[
N = \frac{\partial_u \varphi \times \partial_v \varphi}{\abs{\partial_u \varphi \times \partial_v \varphi}}.
\]

** Examples

*** Sphere:

\[
S = \{x^2 + y^2 + z^2 = 1\}, \quad N(p) = p
\]

\pause

*** Graph:
\[
S = \{(x, y, f(x, y))\}, \quad N(x, y, f(x)) = \frac{1}{\sqrt{1 + f_x^2 + f_y^2}} (-f_x, -f_y, 1).
\]

\pause

*** Inverse image of regular point

\[
S = \{F^{-1}(c)\}, \quad N(p) = \frac{\nabla F(p)}{|\nabla F(p)|}.
\]


